fwd_backwd proof skeleton

Diff/LanguageModel.v
@@ -37,21 +37,21 @@ Structure EventTraceSemantics (L : Language) (Ev : Events) (Es : Endstates) := {
 Coercion ev_semantics : EventTraceSemantics >-> Semantics.
 
 Definition input_totality {L : Language} {Ev : Events} {Es : Endstates}
-                          (is_input : ev Ev -> bool)
+                          (is_input : list (ev Ev) -> bool)
                           (event_semantics : EventTraceSemantics L Ev Es) : Prop :=
-  forall (W : prg L) (l : list (ev Ev)) (i1 i2 : ev Ev),
+  forall (W : prg L) (l i1 i2: list (ev Ev)),
       (is_input i1 = true) ->
       (is_input i1 = true) ->
-      psem event_semantics W (ftbd (snoc l i1)) ->
-      psem event_semantics W ( ftbd (snoc l i2)).  
+      psem event_semantics W (ftbd (l ++ i1)) ->
+      psem event_semantics W (ftbd (l ++ i2)).  
 
 Definition determinacy {L : Language} {Ev : Events} {Es : Endstates}
-                       (is_input : ev Ev -> bool)
+                       (is_input : list (ev Ev) -> bool)
                        (event_semantics : EventTraceSemantics L Ev Es) : Prop :=
   forall (W : prg L) (t1 t2 : @trace Ev Es),
     sem (ev_semantics event_semantics) W t1 ->
     sem (ev_semantics event_semantics) W t2 ->
-    t1 = t2 \/ (exists l i1 i2, i1 <> i2 /\ prefix (ftbd (snoc l i1)) t1 /\ prefix (ftbd (snoc l i2)) t2).  
+    t1 = t2 \/ (exists l i1 i2, i1 <> i2 /\ prefix (ftbd (l ++ i1)) t1 /\ prefix (ftbd (l ++ i2)) t2).  
     
 
 Definition beh {L : Language}
